coq/Syntax.v
@@ -1,9 +1,6 @@
-From Stdlib Require Import Utf8.
-From PolySimpl Require Export Maps.
-From Stdlib Require Export Lists.List Strings.String.
-From Stdlib Require Export ZArith.Int ZArith.
+From Stdlib Require Import Utf8 Strings.String ZArith.
 
-Definition state := total_map Z.
+Definition state := string → Z.
 
 Inductive aexp : Type :=
   | ANum (n : Z)
